BtreeSpec.dfy

examples/MutableBtree.dfy
@@ -27,12 +27,6 @@ abstract module MutableBtree {
   function method DefaultValue() : Value
   function method DefaultKey() : Key
 
-  lemma AssumeFalse()
-    //ensures false
-  {
-    //assert false;
-  }
-
   datatype ImmutableNode =
     | ImmutableLeaf(keys: seq<Key>, values: seq<Value>)
     | ImmutableIndex(pivots: seq<Key>, children: seq<ImmutableNode>)
@@ -102,42 +96,6 @@ abstract module MutableBtree {
     }
   }
 
-  function InsertLeaf(leaf: ImmutableNode, key: Key, value: Value) : (result: ImmutableNode)
-    requires leaf.ImmutableLeaf?
-    requires WFLeaf(leaf)
-    ensures result.ImmutableLeaf?
-    ensures WFLeaf(result)
-  {
-    var llte := Keys.LargestLte(leaf.keys, key);
-    if 0 <= llte && leaf.keys[llte] == key then
-      ImmutableLeaf(leaf.keys, leaf.values[llte := value])
-    else
-      Keys.strictlySortedInsert(leaf.keys, key, llte);
-      ImmutableLeaf(Seq.insert(leaf.keys, key, llte+1), Seq.insert(leaf.values, value, llte+1))
-  }
-
-  lemma InsertLeafIsCorrect(leaf: ImmutableNode, key: Key, value: Value, result: ImmutableNode)
-    requires leaf.ImmutableLeaf?
-    requires WFLeaf(leaf)
-    requires result == InsertLeaf(leaf, key, value)
-    ensures InterpretNode(result) == InterpretNode(leaf)[key := value]
-  {
-    var llte := Keys.LargestLte(leaf.keys, key);
-    if 0 <= llte && leaf.keys[llte] == key {
-      assert InterpretNode(result) == InterpretNode(leaf)[key := value];
-    } else {
-      Keys.reveal_IsStrictlySorted();
-      forall k | k in InterpretNode(result).Keys
-        ensures k in InterpretNode(leaf).Keys + {key}
-      {
-        var kpos := IndexOf(result.keys, k);
-        if llte + 1 < kpos {
-          assert k == leaf.keys[kpos-1];
-        }
-      }
-    }
-  }
-   
   predicate SplitLeaf(oldleaf: ImmutableNode, leftleaf: ImmutableNode, rightleaf: ImmutableNode, pivot: Key)
   {
     && oldleaf.ImmutableLeaf?
@@ -153,15 +111,6 @@ abstract module MutableBtree {
     && Keys.lt(Last(leftleaf.keys), pivot)
     && Keys.lte(pivot, rightleaf.keys[0])
   }
-
-  // lemma SplitLeafAllKeys(oldleaf: ImmutableNode, leftleaf: ImmutableNode, rightleaf: ImmutableNode, pivot: Key)
-  //   requires SplitLeaf(oldleaf, leftleaf, rightleaf, pivot)
-  //   ensures AllKeysNode(oldleaf) == AllKeysNode(leftleaf) + AllKeysNode(rightleaf)
-  //   ensures AllKeysNode(leftleaf) == set k | k in AllKeysNode(oldleaf) && Keys.lt(k, pivot)
-  //   ensures AllKeysNode(rightleaf) == set k | k in AllKeysNode(oldleaf) && Keys.lte(pivot, k)
-  // {
-  //   Keys.reveal_IsStrictlySorted();
-  // }
 
   lemma SplitLeafInterpretation(oldleaf: ImmutableNode, leftleaf: ImmutableNode, rightleaf: ImmutableNode, pivot: Key)
     requires SplitLeaf(oldleaf, leftleaf, rightleaf, pivot)
@@ -197,35 +146,6 @@ abstract module MutableBtree {
     && oldindex.children == leftindex.children + rightindex.children
   }
 
-  // lemma SplitIndexAllKeys(oldindex: ImmutableNode, leftindex: ImmutableNode, rightindex: ImmutableNode, pivot: Key)
-  //   requires SplitIndex(oldindex, leftindex, rightindex, pivot)
-  //   ensures AllKeysNode(oldindex) == AllKeysNode(leftindex) + AllKeysNode(rightindex)
-  //   ensures AllKeysNode(leftindex) == set k | k in AllKeysNode(oldindex) && Keys.lt(k, pivot)
-  //   ensures AllKeysNode(rightindex) == set k | k in AllKeysNode(oldindex) && Keys.lte(pivot, k)
-  // {
-  //   assert AllKeysNode(oldindex) <= AllKeysNode(leftindex) + AllKeysNode(rightindex);
-  //   forall key | key in AllKeysNode(leftindex) + AllKeysNode(rightindex)
-  //     ensures key in AllKeysNode(oldindex)
-  //   {
-  //     if key in AllKeysNode(leftindex) {
-  //       var i :| 0 <= i < |leftindex.children| && key in AllKeysNode(leftindex.children[i]);
-  //       assert key in AllKeysNode(oldindex.children[i]);
-  //     } else {
-  //       var i :| 0 <= i < |rightindex.children| && key in AllKeysNode(rightindex.children[i]);
-  //       assert key in AllKeysNode(oldindex.children[|leftindex.children|+i]);
-  //     }
-  //   }
-  //   forall key | key in AllKeysNode(leftindex)
-  //     ensures Keys.lt(key, pivot)
-  //   {
-      
-  //   }
-  //   assert AllKeysNode(leftindex) <= set k | k in AllKeysNode(oldindex) && Keys.lt(k, pivot);
-  //   assert AllKeysNode(leftindex) >= set k | k in AllKeysNode(oldindex) && Keys.lt(k, pivot);
-  //   assert AllKeysNode(rightindex) <= set k | k in AllKeysNode(oldindex) && Keys.lte(pivot, k);
-  //   assert AllKeysNode(rightindex) >= set k | k in AllKeysNode(oldindex) && Keys.lte(pivot, k);
-  // }
-  
   lemma SplitIndexInterpretation(oldindex: ImmutableNode, leftindex: ImmutableNode, rightindex: ImmutableNode, pivot: Key)
     requires SplitIndex(oldindex, leftindex, rightindex, pivot)
     ensures InterpretIndex(oldindex) == Keys.MapPivotedUnion(InterpretIndex(leftindex), pivot, InterpretIndex(rightindex))
@@ -345,577 +265,601 @@ abstract module MutableBtree {
     }
   }
     
-//   trait Node {
-//     ghost var subtreeObjects: set<object>
-//     ghost var allKeys: set<Key>
+  function InsertLeaf(leaf: ImmutableNode, key: Key, value: Value) : (result: ImmutableNode)
+    requires leaf.ImmutableLeaf?
+    requires WFLeaf(leaf)
+    ensures result.ImmutableLeaf?
+    ensures WFLeaf(result)
+  {
+    var llte := Keys.LargestLte(leaf.keys, key);
+    if 0 <= llte && leaf.keys[llte] == key then
+      ImmutableLeaf(leaf.keys, leaf.values[llte := value])
+    else
+      Keys.strictlySortedInsert(leaf.keys, key, llte);
+      ImmutableLeaf(Seq.insert(leaf.keys, key, llte+1), Seq.insert(leaf.values, value, llte+1))
+  }
 
-//     function ToImmutableNode() : ImmutableNode
-//       reads this, subtreeObjects
-//       decreases subtreeObjects, 0
+  lemma InsertLeafIsCorrect(leaf: ImmutableNode, key: Key, value: Value, result: ImmutableNode)
+    requires leaf.ImmutableLeaf?
+    requires WFLeaf(leaf)
+    requires result == InsertLeaf(leaf, key, value)
+    ensures InterpretNode(result) == InterpretNode(leaf)[key := value]
+  {
+    var llte := Keys.LargestLte(leaf.keys, key);
+    if 0 <= llte && leaf.keys[llte] == key {
+      assert InterpretNode(result) == InterpretNode(leaf)[key := value];
+    } else {
+      Keys.reveal_IsStrictlySorted();
+      forall k | k in InterpretNode(result).Keys
+        ensures k in InterpretNode(leaf).Keys + {key}
+      {
+        var kpos := IndexOf(result.keys, k);
+        if llte + 1 < kpos {
+          assert k == leaf.keys[kpos-1];
+        }
+      }
+    }
+  }
+   
+  trait Node {
+    ghost var subtreeObjects: set<object>
       
-//     predicate WF()
-//       reads this, subtreeObjects
-//       ensures WF() ==> this in subtreeObjects
-//       decreases subtreeObjects, 0
-
-//     // function QueryDef(needle: Key) : QueryResult
-//     //   requires WF()
-//     //   reads this, subtreeObjects
-//     //   decreases subtreeObjects
+    predicate WF()
+      ensures WF() ==> this in subtreeObjects
+      reads this, subtreeObjects
+      decreases subtreeObjects, 0
       
-//     function Interpretation() : map<Key, Value>
-//       requires WF()
-//       // ensures forall key :: QueryDef(key).Found? ==> MapsTo(Interpretation(), key, QueryDef(key).value)
-//       // ensures forall key :: QueryDef(key).NotFound? ==> key !in Interpretation()
-//       reads this, subtreeObjects
-//       decreases subtreeObjects
-
-//     method Query(needle: Key) returns (result: QueryResult)
-//       requires WF()
-//       //ensures result == QueryDef(needle)
-//       ensures needle in Interpretation() ==> result == Found(Interpretation()[needle])
-//       ensures needle !in Interpretation() ==> result == NotFound
-//       decreases subtreeObjects
-
-//     predicate method Full()
-//       requires WF()
-//       reads this, subtreeObjects
+    function ToImmutableNode() : (imnode: ImmutableNode)
+      requires WF()
+      ensures WFNode(imnode)
+      reads this, subtreeObjects
+      decreases subtreeObjects, 2
       
-//     method Insert(key: Key, value: Value)
-//       requires WF()
-//       requires !Full()
-//       ensures WF()
-//       ensures Interpretation() == old(Interpretation())[key := value]
-//       ensures allKeys == old(allKeys) + {key}
-//       ensures fresh(subtreeObjects-old(subtreeObjects))
-//       modifies this, subtreeObjects
-//       decreases allKeys
-      
-//     predicate SplitEnsures(oldint: map<Key, Value>, pivot: Key, rightnode: Node)
-//       reads this, subtreeObjects
-//       reads rightnode, rightnode.subtreeObjects
-//     {
-//       && WF()
-//       && !Full()
-//       && rightnode.WF()
-//       && !rightnode.Full()
-//       && MergeMaps(Interpretation(), pivot, rightnode.Interpretation()) == oldint
-//       && allKeys != {}
-//       && rightnode.allKeys != {}
-//       && (forall key :: key in allKeys ==> Keys.lt(key, pivot))
-//       && (forall key :: key in rightnode.allKeys ==> Keys.lte(pivot, key))
-//     }
-      
-//     method Split() returns (ghost wit: Key, pivot: Key, rightnode: Node)
-//       requires WF()
-//       requires Full()
-//       ensures SplitEnsures(old(Interpretation()), pivot, rightnode)
-//       ensures allKeys <= old(allKeys)
-//       ensures rightnode.allKeys <= old(allKeys)
-//       ensures pivot in old(allKeys)
-//       ensures wit in old(allKeys)
-//       ensures Keys.lt(wit, pivot)
-//       ensures subtreeObjects <= old(subtreeObjects)
-//       ensures subtreeObjects !! rightnode.subtreeObjects
-//       ensures fresh(rightnode.subtreeObjects - old(subtreeObjects))
-//       modifies this
-//   }
+    function AllKeys() : set<Key>
+      requires WF()
+      reads this, subtreeObjects
+      decreases subtreeObjects, 3
+    {
+      AllKeysNode(ToImmutableNode())
+    }
 
-//   datatype NodeBox = NodeBox(node: Node?)
-
-//   class Leaf extends Node {
-//     var nkeys : uint64
-//     var keys: array<Key>
-//     var values: array<Value>
-
-//     function ToImmutableNode() : (result: ImmutableNode)
-//       ensures result.ImmutableLeaf?
-//       reads this, subtreeObjects
-//       decreases subtreeObjects, 0
-//     {
-//       ImmutableLeaf(allKeys, keys[..nkeys], values[..nkeys])
-//     }
+    function Interpretation() : map<Key, Value>
+      requires WF()
+      reads this, subtreeObjects
+      decreases subtreeObjects, 4
+    {
+      InterpretNode(ToImmutableNode())
+    }
     
-//     predicate WF()
-//       reads this, subtreeObjects
-//       ensures WFLEaf() ==> this in subtreeObjects
-//       decreases subtreeObjects, 0
-//     {
-//       && subtreeObjects == {this, keys, values}
-//       && keys != values
-//       && keys.Length == MaxKeysPerLeaf() as int
-//       && values.Length == MaxKeysPerLeaf() as int
-//       && 0 <= nkeys <= keys.Length as uint64
-//       && WFLeaf(ToImmutableNode())
-//     }
+    // method Query(needle: Key) returns (result: QueryResult)
+    //   requires WF()
+    //   ensures needle in Interpretation() ==> result == Found(Interpretation()[needle])
+    //   ensures needle !in Interpretation() ==> result == NotFound
+    //   decreases subtreeObjects
 
-//     function Interpretation() : map<Key, Value>
-//       requires WF()
-//       reads this, subtreeObjects
-//       decreases subtreeObjects
-//     {
-//       InterpretationLeaf(ToImmutableNode())
-//     }
-
-//     method Query(needle: Key) returns (result: QueryResult)
-//       requires WF()
-//       ensures needle in Interpretation() ==> result == Found(Interpretation()[needle])
-//       ensures needle !in Interpretation() ==> result == NotFound
-//       //ensures result == QueryDef(needle)
-//       decreases subtreeObjects
-//     {
-//       //Keys.reveal_IsStrictlySorted();
-//       var posplus1: uint64 := Keys.ArrayLargestLtePlus1(keys, 0, nkeys, needle);
-//       if 1 <= posplus1 && keys[posplus1-1] == needle {
-//         result := Found(values[posplus1-1]);
-//       } else {
-//         result := NotFound;
-//       }
-//     }
-
-//     predicate method Full()
-//       requires WF()
-//       reads this, subtreeObjects
-//     {
-//       nkeys >= MaxKeysPerLeaf()
-//     }
-    
-//     method Insert(key: Key, value: Value)
-//       requires WF()
-//       requires !Full()
-//       ensures WF()
-//       ensures Interpretation() == old(Interpretation())[key := value]
-//       ensures allKeys == old(allKeys) + {key}
-//       ensures fresh(subtreeObjects-old(subtreeObjects))
-//       modifies this, subtreeObjects
-//       decreases allKeys
-//     {
-//       var posplus1 := Keys.ArrayLargestLtePlus1(keys, 0, nkeys, key);
-
-//       if 1 <= posplus1 && keys[posplus1-1] == key {
-//         values[posplus1-1] := value;
-//       } else {
-//         ghost var oldkeys := keys[..nkeys];
-//         Arrays.Insert(keys, nkeys, key, posplus1);
-//         Arrays.Insert(values, nkeys, value, posplus1);
-//         nkeys := nkeys + 1;
-//         allKeys := allKeys + {key};
-
-//         InsertMultiset(oldkeys, key, posplus1 as int); // OBSERVE
-//         Keys.strictlySortedInsert(oldkeys, key, posplus1 as int - 1); // OBSERVE
-//         Keys.PosEqLargestLte(keys[..nkeys], key, posplus1 as int);
-//         forall key' |  key' != key && key' in old(Interpretation())
-//           ensures key' in Interpretation() && Interpretation()[key'] == old(Interpretation())[key']
-//         {
-//           var i: int := Keys.LargestLte(old(keys[..nkeys]), key');
-//           //assert 0 <= i;
-//           if i < posplus1 as int {
-//             //assert keys[i] == key';
-//             Keys.PosEqLargestLte(keys[..nkeys], key', i);
-//           } else {
-//             //assert keys[i+1] == key';
-//             Keys.PosEqLargestLte(keys[..nkeys], key', i+1);
-//           }
-//         }
-//         forall key' | key' != key && key' in Interpretation()
-//           ensures key' in old(Interpretation()) && old(Interpretation())[key'] == Interpretation()[key']
-//         {
-//           var i: int := Keys.LargestLte(keys[..nkeys], key');
-//           if i < posplus1 as int {
-//             Keys.PosEqLargestLte(old(keys[..nkeys]), key', i);
-//           } else {
-//             Keys.PosEqLargestLte(old(keys[..nkeys]), key', i-1);
-//           }
-//         }
-//       }
-//     }
-
-//     method Split() returns (ghost wit: Key, pivot: Key, rightnode: Node)
-//       requires WF()
-//       requires Full()
-//       ensures SplitEnsures(old(Interpretation()), pivot, rightnode)
-//       ensures allKeys <= old(allKeys)
-//       ensures rightnode.allKeys <= old(allKeys)
-//       ensures pivot in old(allKeys)
-//       ensures wit in old(allKeys)
-//       ensures Keys.lt(wit, pivot)
-//       ensures subtreeObjects <= old(subtreeObjects)
-//       ensures subtreeObjects !! rightnode.subtreeObjects
-//       ensures fresh(rightnode.subtreeObjects - old(subtreeObjects))
-//       modifies this
-//     {
-//       var right := new Leaf();
-//       var boundary := nkeys/2;
-//       Arrays.Memcpy(right.keys, 0, keys[boundary..nkeys]); // FIXME: remove conversion to seq
-//       Arrays.Memcpy(right.values, 0, values[boundary..nkeys]); // FIXME: remove conversion to seq
-//       right.nkeys := nkeys - boundary;
-//       nkeys := boundary;
-//       allKeys := set key | key in multiset(keys[..nkeys]);
-//       right.allKeys := set key | key in multiset(right.keys[..right.nkeys]);
-//       assert keys[0] in allKeys;
-//       assert right.keys[0] in right.allKeys;
-//       wit := keys[0];
-//       pivot := right.keys[0];
-//       rightnode := right;
-
-//       assert keys[..nkeys] == old(keys[..nkeys])[..nkeys];
-//       Keys.StrictlySortedSubsequence(old(keys[..nkeys]), 0, nkeys as int);
-//       assert WF();
-//       assert right.keys[..right.nkeys] == old(keys[..nkeys])[boundary..old(nkeys)];
-//       Keys.StrictlySortedSubsequence(old(keys[..nkeys]), boundary as int, old(nkeys) as int);
-//       assert Keys.IsStrictlySorted(right.keys[..right.nkeys]);
-//       assert right.WF();
-//       Keys.IsStrictlySortedImpliesLt(old(keys[..nkeys]), 0, boundary as int);
-//       forall i | 0 <= i < nkeys
-//         ensures Keys.lt(keys[i], pivot)
-//       {
-//         Keys.IsStrictlySortedImpliesLt(old(keys[..nkeys]), i as int, boundary as int);
-//       }
-//       ghost var mergedint := MergeMaps(Interpretation(), pivot, rightnode.Interpretation());
-//       forall key | key in old(Interpretation())
-//         ensures key in mergedint && mergedint[key] == old(Interpretation())[key]
-//       {
-//         if Keys.lt(key, pivot) {
-//           assert Keys.LargestLte(old(keys[..nkeys]), key) < boundary as int;
-//         } else {
-//         }
-//       }
-//     }
+    // predicate method Full()
+    //   requires WF()
+    //   reads this, subtreeObjects
       
-//     constructor()
-//       ensures WF()
-//       ensures Interpretation() == map[]
-//       ensures !Full()
-//       ensures fresh(keys)
-//       ensures fresh(values)
-//     {
-//       nkeys := 0;
-//       keys := new Key[MaxKeysPerLeaf()](_ => DefaultKey());
-//       values := new Value[MaxKeysPerLeaf()](_ => DefaultValue());
-//       allKeys := {};
-//       subtreeObjects := {this, keys, values};
-//     }
-//   }
+    // predicate SplitEnsures(oldint: map<Key, Value>, pivot: Key, rightnode: Node)
+    //   reads this, subtreeObjects
+    //   reads rightnode, rightnode.subtreeObjects
+    // {
+    //   && WF()
+    //   && !Full()
+    //   && rightnode.WF()
+    //   && !rightnode.Full()
+    //   && SplitNode(old(ToImmutableNode()), 
+    //   && Keys.MapPivotedUnion(Interpretation(), pivot, rightnode.Interpretation()) == oldint
+    //   && AllKeys() != {}
+    //   && rightnode.AllKeys() != {}
+    //   && (forall key :: key in AllKeys() ==> Keys.lt(key, pivot))
+    //   && (forall key :: key in rightnode.AllKeys() ==> Keys.lte(pivot, key))
+    // }
+      
+    // method Split() returns (pivot: Key, rightnode: Node)
+    //   requires WF()
+    //   requires Full()
+    //   ensures WF()
+    //   ensures rightnode.WF()
+    //   ensures SplitNode(old(ToImmutableNode()), ToImmutableNode(), rightnode.ToImmutableNode(), pivot)
+    //   ensures !Full()
+    //   ensures !rightnode.Full()
+    //   ensures subtreeObjects <= old(subtreeObjects)
+    //   ensures subtreeObjects !! rightnode.subtreeObjects
+    //   ensures fresh(rightnode.subtreeObjects - old(subtreeObjects))
+    //   modifies this
 
-//   class Index extends Node {
-//     var nchildren: uint64
-//     var pivots: array<Key>
-//     var children: array<NodeBox>
+    // method Insert(key: Key, value: Value)
+    //   requires WF()
+    //   requires !Full()
+    //   ensures WF()
+    //   ensures Interpretation() == old(Interpretation())[key := value]
+    //   ensures AllKeys() == old(AllKeys()) + {key}
+    //   ensures fresh(subtreeObjects-old(subtreeObjects))
+    //   modifies this, subtreeObjects
+    //   decreases AllKeys()
+      
+  }
 
-//     predicate WF()
-//       reads this, subtreeObjects
-//       ensures WF() ==> this in subtreeObjects
-//       decreases subtreeObjects, 0
-//     {
-//       && {this, pivots, children} <= subtreeObjects
-//       && pivots.Length == (MaxChildren() as int) - 1
-//       && children.Length == MaxChildren() as int
-//       && 1 <= nchildren <= MaxChildren()
-//       && (forall i :: 0 <= i < nchildren ==> children[i].node != null)
-//       && (forall i :: 0 <= i < nchildren ==> children[i].node in subtreeObjects)
-//       && (forall i {:trigger children[i].node.subtreeObjects} :: 0 <= i < nchildren as int ==> children[i].node.subtreeObjects < subtreeObjects)
-//       && (forall i {:trigger children[i].node.subtreeObjects} :: 0 <= i < nchildren as int ==> {this, pivots, children} !! children[i].node.subtreeObjects)
-//       && (forall i, j {:trigger children[i].node.subtreeObjects, children[j].node.subtreeObjects} :: 0 <= i < j < nchildren as int ==> children[i].node.subtreeObjects !! children[j].node.subtreeObjects)
-//       && WFIndex(ToImmutableNode())
-//     }
+  datatype NodeBox = NodeBox(node: Node?)
 
-//     // lemma AllKeysStrictlyDecreasing()
-//     //   requires WF()
-//     //   ensures forall i :: 0 <= i < nchildren ==> children[i].node.allKeys < allKeys
-//     // {
-//     //   forall i | 0 <= i < nchildren
-//     //     ensures children[i].node.allKeys < allKeys
-//     //   {
-//     //     var i' := if i < nchildren-1 then i+1 else 0;
-//     //     assert i' != i;
-//     //     assert children[i].node.allKeys !! children[i'].node.allKeys;
-//     //     assert children[i].node.allKeys <= 
-//     //     assert children[i].node.allKeys <= allKeys;
-//     //   }
-//     // }
+  class Leaf extends Node {
+    var nkeys : uint64
+    var keys: array<Key>
+    var values: array<Value>
+
+    predicate WF()
+      ensures WF() ==> this in subtreeObjects
+      reads this, subtreeObjects
+      decreases subtreeObjects, 0
+    {
+      && subtreeObjects == {this, keys, values}
+      && keys != values
+      && keys.Length == MaxKeysPerLeaf() as int
+      && values.Length == MaxKeysPerLeaf() as int
+      && 0 <= nkeys as int <= keys.Length
+      && Keys.IsStrictlySorted(keys[..nkeys])
+    }
+
+    function ToImmutableNode() : (result: ImmutableNode)
+      requires WF()
+      ensures WFNode(result)
+      //ensures result.ImmutableLeaf?
+      reads this, subtreeObjects
+      decreases subtreeObjects, 2
+    {
+      ImmutableLeaf(keys[..nkeys], values[..nkeys])
+    }
     
-//     // function QueryDef(needle: Key) : QueryResult
-//     //   requires WF()
-//     //   reads this, subtreeObjects
-//     //   decreases subtreeObjects
-//     // {
-//     //   var pos := Keys.LargestLte(pivots[..nchildren-1], needle);
-//     //   children[pos + 1].node.QueryDef(needle)
-//     // }
-    
-//     function Interpretation() : (result: map<Key, Value>)
-//       requires WF()
-//       // ensures forall key :: QueryDef(key).Found? ==> MapsTo(result, key, QueryDef(key).value)
-//       // ensures forall key :: QueryDef(key).NotFound? ==> key !in Interpretation()
-//       reads this, subtreeObjects
-//       decreases subtreeObjects
-//     {
-//       // This is just to prove finiteness.  Thanks to James Wilcox for the trick:
-//       // https://stackoverflow.com/a/47585360
-//       var allkeys := set key, i | 0 <= i < nchildren && key in children[i].node.Interpretation() :: key;
-//       var result := map key |
-//         && key in allkeys
-//         && key in children[Keys.LargestLte(pivots[..nchildren-1], key) + 1].node.Interpretation()
-//         :: children[Keys.LargestLte(pivots[..nchildren-1], key) + 1].node.Interpretation()[key];
+    // method Query(needle: Key) returns (result: QueryResult)
+    //   requires WF()
+    //   ensures needle in Interpretation() ==> result == Found(Interpretation()[needle])
+    //   ensures needle !in Interpretation() ==> result == NotFound
+    //   decreases subtreeObjects
+    // {
+    //   //Keys.reveal_IsStrictlySorted();
+    //   var posplus1: uint64 := Keys.ArrayLargestLtePlus1(keys, 0, nkeys, needle);
+    //   if 1 <= posplus1 && keys[posplus1-1] == needle {
+    //     result := Found(values[posplus1-1]);
+    //   } else {
+    //     result := NotFound;
+    //   }
+    // }
 
-//       // assert forall key :: QueryDef(key).Found? ==> key in children[Keys.LargestLte(pivots[..nchildren-1], key)+1].node.Interpretation();
+    // predicate method Full()
+    //   requires WF()
+    //   reads this, subtreeObjects
+    // {
+    //   nkeys >= MaxKeysPerLeaf()
+    // }
+    
+    // method Split() returns (pivot: Key, rightnode: Node)
+    //   requires WF()
+    //   requires Full()
+    //   ensures WF()
+    //   ensures rightnode.WF()
+    //   ensures SplitNode(old(ToImmutableNode()), ToImmutableNode(), rightnode.ToImmutableNode(), pivot)
+    //   ensures !Full()
+    //   ensures !rightnode.Full()
+    //   ensures subtreeObjects <= old(subtreeObjects)
+    //   ensures subtreeObjects !! rightnode.subtreeObjects
+    //   ensures fresh(rightnode.subtreeObjects - old(subtreeObjects))
+    //   modifies this
+    // {
+    //   var right := new Leaf();
+    //   var boundary := nkeys/2;
+    //   Arrays.Memcpy(right.keys, 0, keys[boundary..nkeys]); // FIXME: remove conversion to seq
+    //   Arrays.Memcpy(right.values, 0, values[boundary..nkeys]); // FIXME: remove conversion to seq
+    //   right.nkeys := nkeys - boundary;
+    //   nkeys := boundary;
+    //   pivot := right.keys[0];
+    //   rightnode := right;
+
+    //   assert keys[..nkeys] == old(keys[..nkeys])[..nkeys];
+    //   Keys.StrictlySortedSubsequence(old(keys[..nkeys]), 0, nkeys as int);
+    //   assert right.keys[..right.nkeys] == old(keys[..nkeys])[boundary..old(nkeys)];
+    //   Keys.StrictlySortedSubsequence(old(keys[..nkeys]), boundary as int, old(nkeys) as int);
+    //   Keys.reveal_IsStrictlySorted();
+    //   assert SplitLeaf(old(ToImmutableNode()), ToImmutableNode(), rightnode.ToImmutableNode(), pivot);
+    // }
+      
+    // method Insert(key: Key, value: Value)
+    //   requires WF()
+    //   requires !Full()
+    //   ensures WF()
+    //   ensures Interpretation() == old(Interpretation())[key := value]
+    //   ensures AllKeys() == old(AllKeys()) + {key}
+    //   ensures fresh(subtreeObjects-old(subtreeObjects))
+    //   modifies this, subtreeObjects
+    //   decreases AllKeys()
+    // {
+    //   var posplus1 := Keys.ArrayLargestLtePlus1(keys, 0, nkeys, key);
+
+    //   if 1 <= posplus1 && keys[posplus1-1] == key {
+    //     values[posplus1-1] := value;
+    //   } else {
+    //     ghost var oldkeys := keys[..nkeys];
+    //     Arrays.Insert(keys, nkeys, key, posplus1);
+    //     Arrays.Insert(values, nkeys, value, posplus1);
+    //     nkeys := nkeys + 1;
+
+    //     InsertMultiset(oldkeys, key, posplus1 as int); // OBSERVE
+    //     Keys.strictlySortedInsert(oldkeys, key, posplus1 as int - 1); // OBSERVE
+    //     Keys.PosEqLargestLte(keys[..nkeys], key, posplus1 as int);
+    //     forall key' |  key' != key && key' in old(Interpretation())
+    //       ensures key' in Interpretation() && Interpretation()[key'] == old(Interpretation())[key']
+    //     {
+    //       var i: int := Keys.LargestLte(old(keys[..nkeys]), key');
+    //       //assert 0 <= i;
+    //       if i < posplus1 as int {
+    //         //assert keys[i] == key';
+    //         Keys.PosEqLargestLte(keys[..nkeys], key', i);
+    //       } else {
+    //         //assert keys[i+1] == key';
+    //         Keys.PosEqLargestLte(keys[..nkeys], key', i+1);
+    //       }
+    //     }
+    //     forall key' | key' != key && key' in Interpretation()
+    //       ensures key' in old(Interpretation()) && old(Interpretation())[key'] == Interpretation()[key']
+    //     {
+    //       var i: int := Keys.LargestLte(keys[..nkeys], key');
+    //       if i < posplus1 as int {
+    //         Keys.PosEqLargestLte(old(keys[..nkeys]), key', i);
+    //       } else {
+    //         Keys.PosEqLargestLte(old(keys[..nkeys]), key', i-1);
+    //       }
+    //     }
+    //   }
+    // }
+
+    // constructor()
+    //   ensures WF()
+    //   ensures Interpretation() == map[]
+    //   ensures !Full()
+    //   ensures fresh(keys)
+    //   ensures fresh(values)
+    // {
+    //   nkeys := 0;
+    //   keys := new Key[MaxKeysPerLeaf()](_ => DefaultKey());
+    //   values := new Value[MaxKeysPerLeaf()](_ => DefaultValue());
+    //   subtreeObjects := {this, keys, values};
+    // }
+  }
+
+  class Index extends Node {
+    var nchildren: uint64
+    var pivots: array<Key>
+    var children: array<NodeBox>
+
+    predicate WF()
+      ensures WF() ==> this in subtreeObjects
+      reads this, subtreeObjects
+      decreases subtreeObjects, 0
+    {
+      && {this, pivots, children} <= subtreeObjects
+      && pivots.Length == (MaxChildren() as int) - 1
+      && children.Length == MaxChildren() as int
+      && 1 < nchildren <= MaxChildren()
+      && (forall i :: 0 <= i < nchildren ==> children[i].node != null)
+      && (forall i :: 0 <= i < nchildren ==> children[i].node in subtreeObjects)
+      && (forall i {:trigger children[i].node.subtreeObjects} :: 0 <= i < nchildren as int ==> children[i].node.subtreeObjects < subtreeObjects)
+      && (forall i {:trigger children[i].node.subtreeObjects} :: 0 <= i < nchildren as int ==> {this, pivots, children} !! children[i].node.subtreeObjects)
+      && (forall i, j {:trigger children[i].node.subtreeObjects, children[j].node.subtreeObjects} :: 0 <= i < j < nchildren as int ==> children[i].node.subtreeObjects !! children[j].node.subtreeObjects)
+      
+      && Keys.IsStrictlySorted(pivots[..nchildren-1])
+      && (forall i :: 0 <= i < nchildren ==> children[i].node.WF())
+      && (forall i :: 0 <= i < nchildren ==> children[i].node.AllKeys() != {})
+      && (forall i, key :: 0 <= i < nchildren-1 && key in children[i].node.AllKeys() ==> Keys.lt(key, pivots[i]))
+      && (forall i, key :: 0 < i < nchildren   && key in children[i].node.AllKeys() ==> Keys.lte(pivots[i-1], key))
+    }
+
+    // static function SeqSubtreeObjects(nodes: seq<NodeBox>) : (result: set<object>)
+    //   requires forall i :: 0 <= i < |nodes| ==> nodes[i].node != null
+    //   reads set i | 0 <= i < |nodes| :: nodes[i].node
+    // {
+    //   set i, o | 0 <= i < |nodes| && o in nodes[i].node.subtreeObjects :: o
+    // }
+
+    // lemma SeqSubtreeObjectsDecreasing()
+    //   requires WF()
+    //   requires 1 < nchildren
+    //   ensures forall i :: 0 <= i < nchildren ==> children[i].node.subtreeObjects < SeqSubtreeObjects(children[..nchildren])
+    //   decreases subtreeObjects, 1
+    // {
+    //   forall i | 0 <= i < nchildren
+    //     ensures children[i].node.subtreeObjects < SeqSubtreeObjects(children[..nchildren])
+    //   {
+    //     if 0 < i {
+    //       assert children[i-1].node.WF();
+    //       assert children[i-1].node !in children[i].node.subtreeObjects;
+    //     } else {
+    //       assert children[i+1].node.WF();
+    //       assert children[i+1].node !in children[i].node.subtreeObjects;
+    //     }
+    //   }
+    // }
+    
+    // static function SeqToImmutableNodeSeq(nodes: seq<NodeBox>) : (result: seq<ImmutableNode>)
+    //   requires forall i :: 0 <= i < |nodes| ==> nodes[i].node != null
+    //   requires forall i :: 0 <= i < |nodes| ==> nodes[i].node.subtreeObjects < SeqSubtreeObjects(nodes)
+    //   requires forall i :: 0 <= i < |nodes| ==> nodes[i].node.WF()
+    //   reads set i | 0 <= i < |nodes| :: nodes[i].node
+    //   reads SeqSubtreeObjects(nodes)
+    //   decreases SeqSubtreeObjects(nodes)
+    // {
+    //   if nodes == [] then
+    //     []
+    //   else
+    //     assert Last(nodes).node.subtreeObjects < SeqSubtreeObjects(nodes);
+    //     SeqToImmutableNodeSeq(DropLast(nodes)) + [Last(nodes).node.ToImmutableNode()]
+    // }
+    
+    function ToImmutableNode() : (imnode: ImmutableNode)
+      requires WF()
+      ensures WFNode(imnode)
+      reads this, subtreeObjects
+      decreases subtreeObjects, 2
+    // {
+    //   var impivots := pivots[..nchildren-1];
+    //   SeqSubtreeObjectsDecreasing();
+    //   assert SeqSubtreeObjects(children[..nchildren]) < subtreeObjects;
+    //   var imchildren := SeqToImmutableNodeSeq(children[..nchildren]);
+    //   ImmutableIndex(impivots, imchildren)
+    // }
+    
+    // lemma AllKeysStrictlyDecreasing()
+    //   requires WF()
+    //   ensures forall i :: 0 <= i < nchildren ==> children[i].node.allKeys < allKeys
+    // {
+    //   forall i | 0 <= i < nchildren
+    //     ensures children[i].node.allKeys < allKeys
+    //   {
+    //     var i' := if i < nchildren-1 then i+1 else 0;
+    //     assert i' != i;
+    //     assert children[i].node.allKeys !! children[i'].node.allKeys;
+    //     assert children[i].node.allKeys <= 
+    //     assert children[i].node.allKeys <= allKeys;
+    //   }
+    // }
+    
+    // method Query(needle: Key) returns (result: QueryResult)
+    //   requires WF()
+    //   ensures needle in Interpretation() ==> result == Found(Interpretation()[needle])
+    //   ensures needle !in Interpretation() ==> result == NotFound
+    //   // ensures result == QueryDef(needle)
+    //   decreases subtreeObjects
+    // {
+    //   var posplus1 := Keys.ArrayLargestLtePlus1(pivots, 0, nchildren-1, needle);
+    //   result := children[posplus1].node.Query(needle);
+    // }
+
+    // predicate method Full()
+    //   requires WF()
+    //   reads this, subtreeObjects
+    // {
+    //   nchildren == MaxChildren()
+    // }
+
+    // method SplitChild(key: Key, childidx: uint64)
+    //   requires WF()
+    //   requires !Full()
+    //   requires childidx as int == 1 + Keys.LargestLte(pivots[..nchildren-1], key)
+    //   requires children[childidx].node.Full()
+    //   ensures WF()
+    //   //ensures Interpretation() == old(Interpretation())
+    //   ensures SplitChildOfIndex(old(ToImmutableNode()), ToImmutableNode(), childidx as int)
+    //   ensures fresh(subtreeObjects-old(subtreeObjects))
+    //   modifies this, pivots, children, children[childidx].node
+    // {
+    //   ghost var oldchildren := children;
+      
+    //   var pivot, right := children[childidx].node.Split();
+    //   Arrays.Insert(pivots, nchildren - 1, pivot, childidx);
+    //   Arrays.Insert(children, nchildren, NodeBox(right), childidx + 1);
+    //   nchildren := nchildren + 1;
+    //   subtreeObjects := subtreeObjects + right.subtreeObjects;
+
+      
+    //   // Keys.LargestLteIsUnique(old(pivots[..nchildren-1]), pivot, childidx as int - 1);
+    //   // Keys.strictlySortedInsert(old(pivots[..nchildren-1]), pivot, childidx as int - 1);
+
+    //   assert forall i: uint64 :: 0 <= i < childidx ==> children[i] == oldchildren[i];
+    //   assert children[childidx as int + 1].node == right;
+    //   assert forall i: uint64 :: childidx + 1 < i < nchildren ==> children[i] == oldchildren[i-1];
+    //   // forall i: int, j: int {:trigger children[i].node.subtreeObjects, children[j].node.subtreeObjects}
+    //   // | 0 <= i < j < nchildren as int
+    //   //   ensures children[i].node.subtreeObjects !! children[j].node.subtreeObjects
+    //   // {
+    //   //   if                                   j  < childidx as int {
+    //   //   } else if                            j == childidx as int {
+    //   //   } else if i  < childidx as int     && j == childidx as int + 1 {
+    //   //   } else if i == childidx as int     && j == childidx as int + 1 {
+    //   //   } else if i  < childidx as int     && j  > childidx as int + 1 {
+    //   //   } else if i == childidx as int     && j  > childidx as int + 1 {
+    //   //   } else if i == childidx as int + 1 && j  > childidx as int + 1 {
+    //   //   } else {
+    //   //   }
+    //   // }
+    //   // // forall i: int, key | 0 <= i < (nchildren as int)-1 && key in children[i].node.allKeys
+    //   // //   ensures Keys.lt(key, pivots[i])
+    //   // // {
+    //   // //   if childidx as int + 1 < i {
+    //   // //     assert children[i] == old(children[i-1]);
+    //   // //   }
+    //   // // }
+    //   // // forall i: int, key | 0 < i < nchildren as int && key in children[i].node.allKeys
+    //   // //   ensures Keys.lt(pivots[i-1], key)
+    //   // // {
+    //   // //   if i < childidx as int {
+    //   // //     assert Keys.lt(pivots[i-1], key);
+    //   // //   } else if i == childidx as int {
+    //   // //     assert Keys.lt(pivots[i-1], key);
+    //   // //   } else if i == childidx as int + 1 {
+    //   // //     assert Keys.lt(pivots[i-1], key);
+    //   // //   } else {
+    //   // //     assert Keys.lt(pivots[i-1], key);
+    //   // //   }
+    //   // // }
+    //   // assert WF();
         
-//       result
-//     }
-
-//     method Query(needle: Key) returns (result: QueryResult)
-//       requires WF()
-//       ensures needle in Interpretation() ==> result == Found(Interpretation()[needle])
-//       ensures needle !in Interpretation() ==> result == NotFound
-//       // ensures result == QueryDef(needle)
-//       decreases subtreeObjects
-//     {
-//       var posplus1 := Keys.ArrayLargestLtePlus1(pivots, 0, nchildren-1, needle);
-//       result := children[posplus1].node.Query(needle);
-//     }
-
-//     predicate method Full()
-//       requires WF()
-//       reads this, subtreeObjects
-//     {
-//       nchildren == MaxChildren()
-//     }
-
-//     static lemma SplitChildIsCorrect()
+    //   // forall key | key in old(Interpretation())
+    //   //   ensures key in Interpretation() && Interpretation()[key] == old(Interpretation()[key])
+    //   // {
+    //   //   var llte: int := Keys.LargestLte(old(pivots[..nchildren-1]), key);
+    //   //   assert key in old(children[llte+1].node.Interpretation());
+    //   //   assert old(children[llte+1].node.Interpretation()[key]) == old(Interpretation()[key]);
+    //   //   if llte < childidx as int {
+    //   //     assert key in Interpretation() && Interpretation()[key] == old(Interpretation()[key]);
+    //   //   } else if llte == childidx as int {
+    //   //     if Keys.lt(key, pivot) {
+    //   //       assert key in Interpretation() && Interpretation()[key] == old(Interpretation()[key]);
+    //   //     } else {
+    //   //       assert key in Interpretation() && Interpretation()[key] == old(Interpretation()[key]);
+    //   //     }
+    //   //   } else {
+    //   //     assert key in Interpretation() && Interpretation()[key] == old(Interpretation()[key]);
+    //   //   }
+    //   // }
+    //   // forall key | key in Interpretation()
+    //   //   ensures key in old(Interpretation()) && Interpretation()[key] == old(Interpretation()[key])
+    //   // {
+    //   //   var llte: int := Keys.LargestLte(pivots[..nchildren-1], key);
+    //   //   if llte < childidx as int {
+    //   //   } else if llte == childidx as int {
+    //   //   } else if llte == childidx as int + 1 {
+    //   //   } else {
+    //   //   }
+    //   // }
+    // }
     
-//     method SplitChild(key: Key, childidx: uint64) returns (newchildidx: uint64)
-//       requires WF()
-//       requires !Full()
-//       requires childidx as int == 1 + Keys.LargestLte(pivots[..nchildren-1], key)
-//       requires children[childidx].node.Full()
-//       ensures WF()
-//       ensures Interpretation() == old(Interpretation())
-//       ensures newchildidx as int == 1 + Keys.LargestLte(pivots[..nchildren-1], key)
-//       ensures !children[newchildidx].node.Full()
-//       ensures allKeys == old(allKeys)
-//       ensures fresh(subtreeObjects-old(subtreeObjects))
-//       modifies this, pivots, children, children[childidx].node
-//     {
-//       ghost var oldchildren := children[..nchildren];
-      
-//       var wit, pivot, right := children[childidx].node.Split();
-//       Arrays.Insert(pivots, nchildren - 1, pivot, childidx);
-//       Arrays.Insert(children, nchildren, NodeBox(right), childidx + 1);
-//       nchildren := nchildren + 1;
-//       subtreeObjects := subtreeObjects + right.subtreeObjects;
-//       if Keys.lte(pivot, key) {
-//         newchildidx := childidx + 1;
-//       } else {
-//         newchildidx := childidx;
-//       }
-
-//       Keys.LargestLteIsUnique(old(pivots[..nchildren-1]), pivot, childidx as int - 1);
-//       Keys.strictlySortedInsert(old(pivots[..nchildren-1]), pivot, childidx as int - 1);
-
-//       assert forall i :: 0 <= i < childidx as int ==> children[i] == oldchildren[i];
-//       assert children[childidx as int + 1].node == right;
-//       assert forall i :: childidx as int + 1 < i < nchildren as int  ==> children[i] == oldchildren[i-1];
-//       forall i: int, j: int {:trigger children[i].node.subtreeObjects, children[j].node.subtreeObjects}
-//       | 0 <= i < j < nchildren as int
-//         ensures children[i].node.subtreeObjects !! children[j].node.subtreeObjects
-//       {
-//         if                                   j  < childidx as int {
-//         } else if                            j == childidx as int {
-//         } else if i  < childidx as int     && j == childidx as int + 1 {
-//         } else if i == childidx as int     && j == childidx as int + 1 {
-//         } else if i  < childidx as int     && j  > childidx as int + 1 {
-//         } else if i == childidx as int     && j  > childidx as int + 1 {
-//         } else if i == childidx as int + 1 && j  > childidx as int + 1 {
-//         } else {
-//         }
-//       }
-//       // forall i: int, key | 0 <= i < (nchildren as int)-1 && key in children[i].node.allKeys
-//       //   ensures Keys.lt(key, pivots[i])
-//       // {
-//       //   if childidx as int + 1 < i {
-//       //     assert children[i] == old(children[i-1]);
-//       //   }
-//       // }
-//       // forall i: int, key | 0 < i < nchildren as int && key in children[i].node.allKeys
-//       //   ensures Keys.lt(pivots[i-1], key)
-//       // {
-//       //   if i < childidx as int {
-//       //     assert Keys.lt(pivots[i-1], key);
-//       //   } else if i == childidx as int {
-//       //     assert Keys.lt(pivots[i-1], key);
-//       //   } else if i == childidx as int + 1 {
-//       //     assert Keys.lt(pivots[i-1], key);
-//       //   } else {
-//       //     assert Keys.lt(pivots[i-1], key);
-//       //   }
-//       // }
-//       assert WF();
-        
-//       forall key | key in old(Interpretation())
-//         ensures key in Interpretation() && Interpretation()[key] == old(Interpretation()[key])
-//       {
-//         var llte: int := Keys.LargestLte(old(pivots[..nchildren-1]), key);
-//         assert key in old(children[llte+1].node.Interpretation());
-//         assert old(children[llte+1].node.Interpretation()[key]) == old(Interpretation()[key]);
-//         if llte < childidx as int {
-//           assert key in Interpretation() && Interpretation()[key] == old(Interpretation()[key]);
-//         } else if llte == childidx as int {
-//           if Keys.lt(key, pivot) {
-//             assert key in Interpretation() && Interpretation()[key] == old(Interpretation()[key]);
-//           } else {
-//             assert key in Interpretation() && Interpretation()[key] == old(Interpretation()[key]);
-//           }
-//         } else {
-//           assert key in Interpretation() && Interpretation()[key] == old(Interpretation()[key]);
-//         }
-//       }
-//       forall key | key in Interpretation()
-//         ensures key in old(Interpretation()) && Interpretation()[key] == old(Interpretation()[key])
-//       {
-//         var llte: int := Keys.LargestLte(pivots[..nchildren-1], key);
-//         if llte < childidx as int {
-//         } else if llte == childidx as int {
-//         } else if llte == childidx as int + 1 {
-//         } else {
-//         }
-//       }
-//     }
+    // function UnionSubtreeObjects() : set<object>
+    //   requires nchildren as int <= children.Length
+    //   requires forall i :: 0 <= i < nchildren ==> children[i].node != null
+    //   reads this, children, set i | 0 <= i < nchildren :: children[i].node
+    // {
+    //   set o, i | 0 <= i < nchildren && o in children[i].node.subtreeObjects :: o
+    // }
     
-//     method Insert(key: Key, value: Value)
-//       requires WF()
-//       requires !Full()
-//       ensures WF()
-//       ensures Interpretation() == old(Interpretation())[key := value]
-//       ensures allKeys == old(allKeys) + {key}
-//       ensures fresh(subtreeObjects - old(subtreeObjects))
-//       modifies this, subtreeObjects
-//       decreases allKeys
-//     {
-//       var posplus1 := Keys.ArrayLargestLtePlus1(pivots, 0, nchildren - 1, key);
-//       var childidx := (posplus1) as uint64;
-//       if children[posplus1].node.Full() {
-//         childidx := SplitChild(key, childidx);
-//       }
-//       //AllKeysStrictlyDecreasing();
-//       children[childidx].node.Insert(key, value);
-//       subtreeObjects := subtreeObjects + children[childidx].node.subtreeObjects;
-//       allKeys := allKeys + {key};
-//       forall key' | key' in old(Interpretation()) && key' != key
-//         ensures key' in Interpretation() && Interpretation()[key'] == old(Interpretation()[key'])
-//       {
-//         var i :| 0 <= i < old(nchildren) && key' in old(children[i].node.Interpretation());
-//       }
-      
-//     }
+    // method Split() returns (pivot: Key, rightnode: Node)
+    //   requires WF()
+    //   requires Full()
+    //   ensures WF()
+    //   ensures rightnode.WF()
+    //   ensures SplitNode(old(ToImmutableNode()), ToImmutableNode(), rightnode.ToImmutableNode(), pivot)
+    //   ensures !Full()
+    //   ensures !rightnode.Full()
+    //   ensures subtreeObjects <= old(subtreeObjects)
+    //   ensures subtreeObjects !! rightnode.subtreeObjects
+    //   ensures fresh(rightnode.subtreeObjects - old(subtreeObjects))
+    //   modifies this      
+    // {
+    //   var right := new Index();
+    //   var boundary := nchildren/2;
+    //   Arrays.Memcpy(right.pivots, 0, pivots[boundary..nchildren-1]); // FIXME: remove conversion to seq
+    //   Arrays.Memcpy(right.children, 0, children[boundary..nchildren]); // FIXME: remove conversion to seq
+    //   right.nchildren := nchildren - boundary;
+    //   nchildren := boundary;
+    //   subtreeObjects := {this, pivots, children} + UnionSubtreeObjects();
+    //   right.subtreeObjects := right.subtreeObjects + right.UnionSubtreeObjects();
 
-//     function UnionSubtreeObjects() : set<object>
-//       requires nchildren as int <= children.Length
-//       requires forall i :: 0 <= i < nchildren ==> children[i].node != null
-//       reads this, children, set i | 0 <= i < nchildren :: children[i].node
-//     {
-//       set o, i | 0 <= i < nchildren && o in children[i].node.subtreeObjects :: o
-//     }
+    //   pivot := pivots[boundary-1];
+
+    //   rightnode := right;
+      
+    //   // Keys.reveal_IsStrictlySorted();
+    //   // assert WF();
+    //   // assert rightnode.WF();
+    //   // assert MergeMaps(Interpretation(), pivot, rightnode.Interpretation()) == old(Interpretation());
+    // }
+
+    // // method Insert(key: Key, value: Value)
+    // //   requires WF()
+    // //   requires !Full()
+    // //   ensures WF()
+    // //   ensures Interpretation() == old(Interpretation())[key := value]
+    // //   ensures allKeys == old(allKeys) + {key}
+    // //   ensures fresh(subtreeObjects - old(subtreeObjects))
+    // //   modifies this, subtreeObjects
+    // //   decreases allKeys
+    // // {
+    // //   var posplus1 := Keys.ArrayLargestLtePlus1(pivots, 0, nchildren - 1, key);
+    // //   var childidx := (posplus1) as uint64;
+    // //   if children[posplus1].node.Full() {
+    // //     childidx := SplitChild(key, childidx);
+    // //   }
+    // //   //AllKeysStrictlyDecreasing();
+    // //   children[childidx].node.Insert(key, value);
+    // //   subtreeObjects := subtreeObjects + children[childidx].node.subtreeObjects;
+    // //   allKeys := allKeys + {key};
+    // //   forall key' | key' in old(Interpretation()) && key' != key
+    // //     ensures key' in Interpretation() && Interpretation()[key'] == old(Interpretation()[key'])
+    // //   {
+    // //     var i :| 0 <= i < old(nchildren) && key' in old(children[i].node.Interpretation());
+    // //   }
+      
+    // // }
+
+    // constructor()
+    //   ensures nchildren == 0
+    //   ensures pivots.Length == (MaxChildren() as int)-1
+    //   ensures children.Length == (MaxChildren() as int)
+    //   ensures forall i :: 0 <= i < children.Length ==> children[i].node == null
+    //   ensures subtreeObjects == {this, pivots, children}
+    //   ensures fresh(pivots)
+    //   ensures fresh(children)
+    // {
+    //   pivots := new Key[MaxChildren()-1](_ => DefaultKey());
+    //   children := new NodeBox[MaxChildren()](_ => NodeBox(null));
+    //   nchildren := 0;
+    //   subtreeObjects := {this, pivots, children};
+    // }
+  }
+
+  // class MutableBtree {
+  //   var root: Node
+
+  //   function Interpretation() : map<Key, Value>
+  //     requires root.WF()
+  //     reads this, root, root.subtreeObjects
+  //   {
+  //     root.Interpretation()
+  //   }
+
+  //   method Query(needle: Key) returns (result: QueryResult)
+  //     requires root.WF()
+  //     ensures result == NotFound ==> needle !in Interpretation()
+  //     ensures result.Found? ==> needle in Interpretation() && Interpretation()[needle] == result.value
+  //   {
+  //     result := root.Query(needle);
+  //   }
+
+  //   method Insert(key: Key, value: Value)
+  //     requires root.WF()
+  //     ensures root.WF()
+  //     ensures Interpretation() == old(Interpretation())[key := value]
+  //     modifies this, root, root.subtreeObjects
+  //   {
+  //     if root.Full() {
+  //       var newroot := new Index();
+  //       newroot.children[0] := NodeBox(root);
+  //       newroot.nchildren := 1;
+  //       newroot.subtreeObjects := newroot.subtreeObjects + root.subtreeObjects;
+  //       newroot.allKeys := root.allKeys;
+  //       root := newroot;
+  //     }
+  //     AssumeFalse();
+  //     root.Insert(key, value);
+  //   }
     
-//     method Split() returns (ghost wit: Key, pivot: Key, rightnode: Node)
-//       requires WF()
-//       requires Full()
-//       ensures SplitEnsures(old(Interpretation()), pivot, rightnode)
-//       ensures allKeys <= old(allKeys)
-//       ensures rightnode.allKeys <= old(allKeys)
-//       ensures pivot in old(allKeys)
-//       ensures wit in old(allKeys)
-//       ensures Keys.lt(wit, pivot)
-//       ensures subtreeObjects <= old(subtreeObjects)
-//       ensures subtreeObjects !! rightnode.subtreeObjects
-//       ensures fresh(rightnode.subtreeObjects - old(subtreeObjects))
-//       modifies this
-//     {
-//       var right := new Index();
-//       var boundary := nchildren/2;
-//       Arrays.Memcpy(right.pivots, 0, pivots[boundary..nchildren-1]); // FIXME: remove conversion to seq
-//       Arrays.Memcpy(right.children, 0, children[boundary..nchildren]); // FIXME: remove conversion to seq
-//       right.nchildren := nchildren - boundary;
-//       nchildren := boundary;
-//       subtreeObjects := {this, pivots, children} + UnionSubtreeObjects();
-//       right.subtreeObjects := right.subtreeObjects + right.UnionSubtreeObjects();
-
-//       pivot := pivots[boundary-1];
-
-//       right.allKeys := set k | k in allKeys && Keys.lte(pivot, k);
-//       allKeys := set k | k in allKeys && Keys.lt(k, pivot);
-      
-//       wit := right.pivots[0];
-//       rightnode := right;
-//       AssumeFalse();
-      
-//       // Keys.reveal_IsStrictlySorted();
-//       // assert WF();
-//       // assert rightnode.WF();
-//       // assert MergeMaps(Interpretation(), pivot, rightnode.Interpretation()) == old(Interpretation());
-//     }
-
-//     constructor()
-//       ensures nchildren == 0
-//       ensures pivots.Length == (MaxChildren() as int)-1
-//       ensures children.Length == (MaxChildren() as int)
-//       ensures forall i :: 0 <= i < children.Length ==> children[i].node == null
-//       ensures subtreeObjects == {this, pivots, children}
-//       ensures allKeys == {}
-//       ensures fresh(pivots)
-//       ensures fresh(children)
-//     {
-//       pivots := new Key[MaxChildren()-1](_ => DefaultKey());
-//       children := new NodeBox[MaxChildren()](_ => NodeBox(null));
-//       nchildren := 0;
-//       subtreeObjects := {this, pivots, children};
-//       allKeys := {};
-//     }
-//   }
-
-//   class MutableBtree {
-//     var root: Node
-
-//     function Interpretation() : map<Key, Value>
-//       requires root.WF()
-//       reads this, root, root.subtreeObjects
-//     {
-//       root.Interpretation()
-//     }
-
-//     method Query(needle: Key) returns (result: QueryResult)
-//       requires root.WF()
-//       ensures result == NotFound ==> needle !in Interpretation()
-//       ensures result.Found? ==> needle in Interpretation() && Interpretation()[needle] == result.value
-//     {
-//       result := root.Query(needle);
-//     }
-
-//     method Insert(key: Key, value: Value)
-//       requires root.WF()
-//       ensures root.WF()
-//       ensures Interpretation() == old(Interpretation())[key := value]
-//       modifies this, root, root.subtreeObjects
-//     {
-//       if root.Full() {
-//         var newroot := new Index();
-//         newroot.children[0] := NodeBox(root);
-//         newroot.nchildren := 1;
-//         newroot.subtreeObjects := newroot.subtreeObjects + root.subtreeObjects;
-//         newroot.allKeys := root.allKeys;
-//         root := newroot;
-//       }
-//       AssumeFalse();
-//       root.Insert(key, value);
-//     }
-    
-//     constructor()
-//       ensures root.WF()
-//       ensures Interpretation() == map[]
-//     {
-//       root := new Leaf();
-//     }
-//   }
-// }
+  //   constructor()
+  //     ensures root.WF()
+  //     ensures Interpretation() == map[]
+  //   {
+  //     root := new Leaf();
+  //   }
+  // }
+}
 
 // module TestMutableBtree refines MutableBtree {
 //   import Keys = Uint64_Order
@@ -979,4 +923,4 @@ abstract module MutableBtree {
 //   // }
 //     print "PASSED\n";
 //   }
-} 
+// } 
