examples/BtreeSpec.dfy
@@ -1,0 +1,374 @@
+include "../lib/sequences.dfy"
+include "../lib/Maps.dfy"
+include "../lib/total_order.dfy"
+
+abstract module BtreeSpec {
+  import opened Seq = Sequences
+  import opened Maps
+  import Keys : Total_Order
+
+  type Key = Keys.Element
+  type Value
+    
+  datatype QueryResult =
+    | Found(value: Value)
+    | NotFound
+    
+  datatype Node =
+    | Leaf(keys: seq<Key>, values: seq<Value>)
+    | Index(pivots: seq<Key>, children: seq<Node>)
+
+  function LocalKeys(node: Node) : set<Key>
+  {
+    match node {
+      case Leaf(keys, values) => set k | k in keys
+      case Index(pivots, children) => set k | k in pivots
+    }    
+  }    
+    
+  function AllKeys(node: Node) : set<Key>
+  {
+    match node {
+      case Leaf(keys, values) => set k | k in keys
+      case Index(pivots, children) => set i, k | 0 <= i < |children| && k in AllKeys(children[i]) :: k
+    }    
+  }
+  
+  predicate WFLeaf(leaf: Node)
+    requires leaf.Leaf?
+  {
+    && |leaf.keys| == |leaf.values|
+    && Keys.IsStrictlySorted(leaf.keys)
+  }
+
+  predicate WFIndex(index: Node)
+    requires index.Index?
+    decreases index, 0
+  {
+    && |index.pivots| == |index.children| - 1
+    && Keys.IsStrictlySorted(index.pivots)
+    && (forall i :: 0 <= i < |index.children| ==> WF(index.children[i]))
+    && (forall i :: 0 <= i < |index.children| ==> LocalKeys(index.children[i]) != {})
+    && (forall i, key :: 0 <= i < |index.children|-1 && key in LocalKeys(index.children[i]) ==> Keys.lt(key, index.pivots[i]))
+    && (forall i, key :: 0 < i < |index.children|   && key in LocalKeys(index.children[i]) ==> Keys.lte(index.pivots[i-1], key))
+  }
+
+  predicate WF(node: Node)
+    decreases node, 1
+  {
+    match node {
+      case Leaf(_, _) =>  WFLeaf(node)
+      case Index(_, _) => WFIndex(node)
+    }
+  }
+
+  function InterpretLeaf(leaf: Node) : map<Key, Value>
+    requires leaf.Leaf?
+    requires WFLeaf(leaf)
+  {
+    Keys.PosEqLargestLteForAllElts(leaf.keys);
+    map k | (k in leaf.keys) :: leaf.values[Keys.LargestLte(leaf.keys, k)]
+  }
+
+  function InterpretIndex(index: Node) : map<Key, Value>
+    requires index.Index?
+    requires WFIndex(index)
+    decreases index, 0
+  {
+    map key |
+      && key in AllKeys(index)
+      && key in InterpretNode(index.children[Keys.LargestLte(index.pivots, key) + 1])
+      :: InterpretNode(index.children[Keys.LargestLte(index.pivots, key) + 1])[key]
+  }
+
+  function InterpretNode(node: Node) : map<Key, Value>
+    requires WF(node)
+    decreases node, 1
+  {
+    match node {
+      case Leaf(_, _) => InterpretLeaf(node)
+      case Index(_, _) => InterpretIndex(node)
+    }
+  }
+
+  lemma AllKeysIsConsistentWithInterpretation(node: Node, key: Key)
+    requires WF(node)
+    requires key in InterpretNode(node)
+    ensures node.Index? ==> key in AllKeys(node.children[Keys.LargestLte(node.pivots, key) + 1])
+  {
+    if node.Index? {
+      assert key in InterpretNode(node.children[Keys.LargestLte(node.pivots, key) + 1]);
+    }
+  }
+  
+  lemma AllKeysIsConsistentWithInterpretationUniversal(node: Node)
+    requires WF(node)
+    requires node.Index?
+    ensures forall key :: key in InterpretNode(node) ==> key in AllKeys(node.children[Keys.LargestLte(node.pivots, key) + 1])
+  {
+    forall key | key in InterpretNode(node)
+      ensures key in AllKeys(node.children[Keys.LargestLte(node.pivots, key) + 1])
+    {
+      AllKeysIsConsistentWithInterpretation(node, key);
+    }
+  }
+  
+  predicate SplitLeaf(oldleaf: Node, leftleaf: Node, rightleaf: Node, pivot: Key)
+  {
+    && oldleaf.Leaf?
+    && leftleaf.Leaf?
+    && rightleaf.Leaf?
+    && WFLeaf(oldleaf)
+    && WFLeaf(leftleaf)
+    && WFLeaf(rightleaf)
+    && 0 < |leftleaf.keys|
+    && 0 < |rightleaf.keys|
+    && oldleaf.keys == leftleaf.keys + rightleaf.keys
+    && oldleaf.values == leftleaf.values + rightleaf.values
+    && Keys.lt(Last(leftleaf.keys), pivot)
+    && Keys.lte(pivot, rightleaf.keys[0])
+  }
+
+  lemma SplitLeafInterpretation(oldleaf: Node, leftleaf: Node, rightleaf: Node, pivot: Key)
+    requires SplitLeaf(oldleaf, leftleaf, rightleaf, pivot)
+    ensures InterpretLeaf(oldleaf) == MapDisjointUnion(InterpretLeaf(leftleaf), InterpretLeaf(rightleaf))
+  {
+    var oldint := InterpretLeaf(oldleaf);
+    var leftint := InterpretLeaf(leftleaf);
+    var rightint := InterpretLeaf(rightleaf);
+    var newint := MapDisjointUnion(leftint, rightint);
+
+    forall key | key in oldint
+      ensures newint[key] == oldint[key]
+    {
+      var llte := Keys.LargestLte(oldleaf.keys, key);
+      if llte < |leftleaf.keys| {
+        Keys.PosEqLargestLte(leftleaf.keys, key, llte);
+      } else {
+        var rightllte := llte - |leftleaf.keys|;
+        Keys.PosEqLargestLte(rightleaf.keys, key, rightllte);
+      }
+    }
+  }
+  
+  predicate SplitIndex(oldindex: Node, leftindex: Node, rightindex: Node, pivot: Key)
+  {
+    && oldindex.Index?
+    && leftindex.Index?
+    && rightindex.Index?
+    && WFIndex(oldindex)
+    && WFIndex(leftindex)
+    && WFIndex(rightindex)
+    && oldindex.pivots == leftindex.pivots + [pivot] + rightindex.pivots
+    && oldindex.children == leftindex.children + rightindex.children
+  }
+
+  lemma SplitIndexInterpretation(oldindex: Node, leftindex: Node, rightindex: Node, pivot: Key)
+    requires SplitIndex(oldindex, leftindex, rightindex, pivot)
+    ensures InterpretIndex(oldindex) == Keys.MapPivotedUnion(InterpretIndex(leftindex), pivot, InterpretIndex(rightindex))
+  {
+    var oldint := InterpretIndex(oldindex);
+    var leftint := InterpretIndex(leftindex);
+    var rightint := InterpretIndex(rightindex);
+    var newint := Keys.MapPivotedUnion(leftint, pivot, rightint);
+
+    Keys.reveal_IsStrictlySorted();
+    Keys.PosEqLargestLte(oldindex.pivots, pivot, |leftindex.pivots|);
+    
+    forall key | key in oldint
+      ensures MapsTo(newint, key, oldint[key])
+    {
+      AllKeysIsConsistentWithInterpretation(oldindex, key);
+    }
+
+    forall key | key in newint
+      ensures MapsTo(oldint, key, newint[key])
+    {
+      if Keys.lt(key, pivot) {
+        AllKeysIsConsistentWithInterpretation(leftindex, key);
+        var llte := Keys.LargestLte(leftindex.pivots, key);
+        assert oldindex.children[llte+1] == leftindex.children[llte+1];
+      } else {
+        AllKeysIsConsistentWithInterpretation(rightindex, key);
+        var llte := Keys.LargestLte(rightindex.pivots, key);
+        assert oldindex.children[|leftindex.children| + llte + 1] == rightindex.children[llte+1];
+      }
+    }
+    
+  }
+  
+  predicate SplitNode(oldnode: Node, leftnode: Node, rightnode: Node, pivot: Key)
+  {
+    || SplitLeaf(oldnode, leftnode, rightnode, pivot)
+    || SplitIndex(oldnode, leftnode, rightnode, pivot)
+  }
+
+  lemma SplitNodeInterpretation(oldnode: Node, leftnode: Node, rightnode: Node, pivot: Key)
+    requires SplitNode(oldnode, leftnode, rightnode, pivot)
+    ensures InterpretNode(oldnode) == Keys.MapPivotedUnion(InterpretNode(leftnode), pivot, InterpretNode(rightnode))
+  {
+    if SplitLeaf(oldnode, leftnode, rightnode, pivot) {
+      SplitLeafInterpretation(oldnode, leftnode, rightnode, pivot);
+    } else {
+      SplitIndexInterpretation(oldnode, leftnode, rightnode, pivot);
+    }
+  }
+
+  lemma SplitNodeAllKeys(oldnode: Node, leftnode: Node, rightnode: Node, pivot: Key)
+    requires SplitNode(oldnode, leftnode, rightnode, pivot)
+    ensures AllKeys(oldnode) == AllKeys(leftnode) + AllKeys(rightnode)
+  {
+    if SplitLeaf(oldnode, leftnode, rightnode, pivot) {
+    } else {
+      forall key | key in AllKeys(leftnode) + AllKeys(rightnode)
+        ensures key in AllKeys(oldnode)
+      {
+        if key in AllKeys(leftnode) {
+          var i :| 0 <= i < |leftnode.children| && key in AllKeys(leftnode.children[i]);
+          assert oldnode.children[i] == leftnode.children[i];
+        } else {
+          var i :| 0 <= i < |rightnode.children| && key in AllKeys(rightnode.children[i]);
+          assert oldnode.children[i + |leftnode.children|] == rightnode.children[i];
+        }
+      }
+    }
+  }
+  
+  predicate SplitChildOfIndex(oldindex: Node, newindex: Node, childidx: int)
+  {
+    && oldindex.Index?
+    && newindex.Index?
+    && WF(oldindex)
+    && WF(newindex)
+    && 0 <= childidx < |oldindex.children|
+    && |newindex.children| == |oldindex.children| + 1 // FIXME: WTF?  Dafny can't get these from WF?
+    && |newindex.pivots| == |oldindex.pivots| + 1
+    && |oldindex.pivots| == |oldindex.children| - 1
+    && newindex.pivots == Seq.insert(oldindex.pivots, newindex.pivots[childidx], childidx)
+    && SplitNode(oldindex.children[childidx], newindex.children[childidx], newindex.children[childidx+1], newindex.pivots[childidx])
+    && newindex.children == oldindex.children[..childidx] + [newindex.children[childidx], newindex.children[childidx+1]] + oldindex.children[childidx+1..]
+  }
+
+  lemma SplitChildOfIndexPreservesAllKeys(oldindex: Node, newindex: Node, childidx: int)
+    requires SplitChildOfIndex(oldindex, newindex, childidx)
+    ensures AllKeys(newindex) == AllKeys(oldindex)
+  {
+    assert WFIndex(oldindex);
+    assert WFIndex(newindex);
+    
+    forall key | key in AllKeys(oldindex)
+      ensures key in AllKeys(newindex)
+    {
+      var i :| 0 <= i < |oldindex.children| && key in AllKeys(oldindex.children[i]);
+      if i < childidx {
+      } else if i == childidx {
+        SplitNodeAllKeys(oldindex.children[childidx], newindex.children[childidx], newindex.children[childidx+1], newindex.pivots[childidx]);
+      } else {
+        assert newindex.children[i+1] == oldindex.children[i];
+      }
+    }
+    
+    forall key | key in AllKeys(newindex)
+      ensures key in AllKeys(oldindex)
+    {
+      var i :| 0 <= i < |newindex.children| && key in AllKeys(newindex.children[i]);
+      if i < childidx {
+      } else if i == childidx {
+        SplitNodeAllKeys(oldindex.children[childidx], newindex.children[childidx], newindex.children[childidx+1], newindex.pivots[childidx]);
+      } else if i == childidx + 1 {
+        SplitNodeAllKeys(oldindex.children[childidx], newindex.children[childidx], newindex.children[childidx+1], newindex.pivots[childidx]);
+      } else {
+      }
+    }
+  }
+  
+  lemma SplitChildOfIndexPreservesInterpretation(oldindex: Node, newindex: Node, childidx: int)
+    requires SplitChildOfIndex(oldindex, newindex, childidx)
+    ensures InterpretNode(newindex) == InterpretNode(oldindex)
+  {
+    var newint := InterpretNode(newindex);
+    var oldint := InterpretNode(oldindex);
+
+    // WTF?  Dafny can't see these (from emacs flycheck mode)
+    assert WFIndex(oldindex);
+    assert WFIndex(newindex);
+    assert oldint == InterpretIndex(oldindex);
+    assert newint == InterpretIndex(newindex);
+    
+    var oldchild := oldindex.children[childidx];
+    var leftchild := newindex.children[childidx];
+    var rightchild := newindex.children[childidx+1];
+    var pivot := newindex.pivots[childidx];
+    SplitNodeInterpretation(oldchild, leftchild, rightchild, pivot);        
+    SplitChildOfIndexPreservesAllKeys(oldindex, newindex, childidx);
+    
+    forall key | key in oldint
+      ensures key in newint && newint[key] == oldint[key]
+    {
+      var llte := Keys.LargestLte(oldindex.pivots, key);
+      if llte + 1 < childidx {
+        assert llte == Keys.LargestLte(newindex.pivots, key);
+      } else if llte + 1 == childidx {
+      } else {
+        var newllte := llte + 1;
+        assert newllte == Keys.LargestLte(newindex.pivots, key);
+        assert newindex.children[newllte+1] == oldindex.children[llte+1];
+      }
+    }
+
+    forall key | key in newint
+      ensures key in oldint
+    {
+      var llte := Keys.LargestLte(newindex.pivots, key);
+      if llte + 1 < childidx {
+        assert llte == Keys.LargestLte(oldindex.pivots, key);
+      } else if llte + 1 == childidx {
+        var oldllte := llte;
+        assert oldllte == Keys.LargestLte(oldindex.pivots, key);
+        assert key in InterpretNode(oldindex.children[Keys.LargestLte(oldindex.pivots, key) + 1]);
+      } else if llte + 1 == childidx + 1 {
+        var oldllte := llte - 1;
+        assert oldllte == Keys.LargestLte(oldindex.pivots, key);
+        assert key in InterpretNode(oldindex.children[Keys.LargestLte(oldindex.pivots, key) + 1]);
+      } else {
+        assert llte - 1 == Keys.LargestLte(oldindex.pivots, key);
+      }
+    }
+  }
+    
+  function InsertLeaf(leaf: Node, key: Key, value: Value) : (result: Node)
+    requires leaf.Leaf?
+    requires WFLeaf(leaf)
+    ensures result.Leaf?
+    ensures WFLeaf(result)
+  {
+    var llte := Keys.LargestLte(leaf.keys, key);
+    if 0 <= llte && leaf.keys[llte] == key then
+      Leaf(leaf.keys, leaf.values[llte := value])
+    else
+      Keys.strictlySortedInsert(leaf.keys, key, llte);
+      Leaf(Seq.insert(leaf.keys, key, llte+1), Seq.insert(leaf.values, value, llte+1))
+  }
+
+  lemma InsertLeafIsCorrect(leaf: Node, key: Key, value: Value, result: Node)
+    requires leaf.Leaf?
+    requires WFLeaf(leaf)
+    requires result == InsertLeaf(leaf, key, value)
+    ensures InterpretNode(result) == InterpretNode(leaf)[key := value]
+  {
+    var llte := Keys.LargestLte(leaf.keys, key);
+    if 0 <= llte && leaf.keys[llte] == key {
+      assert InterpretNode(result) == InterpretNode(leaf)[key := value];
+    } else {
+      Keys.reveal_IsStrictlySorted();
+      forall k | k in InterpretNode(result).Keys
+        ensures k in InterpretNode(leaf).Keys + {key}
+      {
+        var kpos := IndexOf(result.keys, k);
+        if llte + 1 < kpos {
+          assert k == leaf.keys[kpos-1];
+        }
+      }
+    }
+  }
+}
